src/Examples/Interval/Ctx/Example_Interval_DG_Ctx_Collect.thy
@@ -40,8 +40,8 @@ definition ivl_ctx_sg :: "pp \<times> ivl + gk \<Rightarrow> ivl abs_state" wher
      (case k of
         Inl (v, ctx) \<Rightarrow>
           (if (v, ctx) \<in> fst twice_ctx_sol
-           then locals ((fun_of_dg_st \<circ> snd twice_ctx_sol) (Inl (v, ctx)))
-                \<squnion> globs ((fun_of_dg_st \<circ> snd twice_ctx_sol) (Inr Global))
+           then locals ((fun_of_dg_st_for twice_gs \<circ> snd twice_ctx_sol) (Inl (v, ctx)))
+                \<squnion> globs ((fun_of_dg_st_for twice_gs \<circ> snd twice_ctx_sol) (Inr Global))
            else bot)
       | Inr _ \<Rightarrow> bot)"
 
@@ -55,12 +55,13 @@ text \<open>One name for the transported abstract solution and the abstract rout
   again inside a semantic obligation.\<close>
 
 abbreviation sigma_abs :: "pp \<times> ivl + gk \<Rightarrow> (ivl abs_state, ivl abs_state) dg_state" where
-  "sigma_abs \<equiv> fun_of_dg_st \<circ> snd twice_ctx_sol"
+  "sigma_abs \<equiv> fun_of_dg_st_for twice_gs \<circ> snd twice_ctx_sol"
 
 abbreviation gen_abs :: "(pp \<times> ivl, gk, (ivl abs_state, ivl abs_state) dg_state) eqsT" where
   "gen_abs \<equiv> side_cfg_T_eff_keyed_seed_dg intra_predecessor_list (\<lambda>_. Global) route_abs_gen
        (routed_cmb Sabs Global) (routed_extra twice_cfg Sabs Seed Global) twice_cfg Sabs
-       (fun_of_exec_dg_st (bot::ivl exec_dg_st)) (fun_of_exec_dg_st cinit_ivl_st) (fun_of_exec_dg_st (restrict_global_resolved_q cinit_ivl_st))"
+       (fun_of_exec_dg_st_for twice_gs (bot::ivl exec_dg_st)) (fun_of_exec_dg_st_for twice_gs cinit_ivl_st)
+       (fun_of_exec_dg_st_for twice_gs (restrict_global_resolved_q cinit_ivl_st))"
 
 lemma pp_eq_bound:
   "(v, ctx) \<in> fst twice_ctx_sol
@@ -94,9 +95,9 @@ qed simp
 text \<open>The entry local slot dominates the initial abstract store \<open>s0d\<close>.\<close>
 lemma entry_locals_ge_s0d:
   assumes cov: "(cfg_entry twice_cfg, bot) \<in> fst twice_ctx_sol"
-  shows "fun_of_exec_dg_st cinit_ivl_st \<le> locals (sigma_abs (Inl (cfg_entry twice_cfg, bot)))"
+  shows "fun_of_exec_dg_st_for twice_gs cinit_ivl_st \<le> locals (sigma_abs (Inl (cfg_entry twice_cfg, bot)))"
 proof -
-  have "fun_of_exec_dg_st cinit_ivl_st \<le> locals (eq gen_abs (cfg_entry twice_cfg, bot) sigma_abs)"
+  have "fun_of_exec_dg_st_for twice_gs cinit_ivl_st \<le> locals (eq gen_abs (cfg_entry twice_cfg, bot) sigma_abs)"
     by (simp add: eq_side_cfg_T_eff_keyed_seed_dg)
        (rule order_trans[OF _ side_acc_dg_ge], simp add: le_supI2)
   also have "\<dots> \<le> locals (sigma_abs (Inl (cfg_entry twice_cfg, bot)))"
@@ -107,8 +108,8 @@ qed
 lemma entry_covered: "(cfg_entry twice_cfg, bot) \<in> fst twice_ctx_sol"
   unfolding twice_ctx_sol_def twice_ctx_eqs_def Spoly_def by eval
 
-lemma cinit_le_cinit_ivl_st: "cinit_stores is_global \<subseteq> \<lbrakk>fun_of_exec_dg_st cinit_ivl_st\<rbrakk>"
-  by (auto simp: cinit_stores_def gamma_state_def fun_of_st_cinit_ivl_st)
+lemma cinit_le_cinit_ivl_st: "cinit_stores twice_gs \<subseteq> \<lbrakk>fun_of_exec_dg_st_for twice_gs cinit_ivl_st\<rbrakk>"
+  by (auto simp: cinit_stores_def gamma_state_def fun_of_exec_dg_st_for_def fun_of_st_cinit_ivl_st_for)
 
 text \<open>
   \<^bold>\<open>Regression: the callee entry stays absent at the root context.\<close>  \<^const>\<open>cfg_entry\<close>
@@ -123,7 +124,7 @@ text \<open>
   keep that invariant honest.\<close>
 
 lemma callee_entry_bot_unpopulated:
-  "lookup_exec_dg_st (locals (snd twice_ctx_sol (Inl (FunctionEntry ''twice'', bot)))) ''p'' = \<bottom>"
+  "twice_lookup_exec_dg_st (locals (snd twice_ctx_sol (Inl (FunctionEntry ''twice'', bot)))) ''p'' = \<bottom>"
   unfolding twice_ctx_sol_def twice_ctx_eqs_def Spoly_def by eval
 
 lemma main_first_stmt_is_call:
@@ -158,9 +159,14 @@ text \<open>The routed interval solution is a \<^locale>\<open>dg_ctx_activation
   and the combine transport are then read off as \<open>twice_dg.dg_ctx_act_edge\<close> /
   \<open>twice_dg.dg_ctx_act_comb_covered\<close> rather than re-proved by hand.\<close>
 
-interpretation twice_dg: dg_ctx_activation Sabs is_global twice_cfg Global route_abs_gen
+text \<open>\<open>ivl_dg_for\<close> (\<open>Example_Interval_DG_Ctx_Sound\<close>) already establishes
+  \<^locale>\<open>sound_dg_spec\<close> \<open>Sabs gamma_unit twice_gs\<close>, so the obligations
+  \<open>dg_ctx_activation\<close> inherits from it discharge automatically below.\<close>
+
+interpretation twice_dg: dg_ctx_activation Sabs twice_gs twice_cfg Global route_abs_gen
     "routed_cmb Sabs Global" "routed_extra twice_cfg Sabs Seed Global"
-    "fun_of_exec_dg_st (bot::ivl exec_dg_st)" "fun_of_exec_dg_st cinit_ivl_st" "fun_of_exec_dg_st (restrict_global_resolved_q cinit_ivl_st)"
+    "fun_of_exec_dg_st_for twice_gs (bot::ivl exec_dg_st)" "fun_of_exec_dg_st_for twice_gs cinit_ivl_st"
+    "fun_of_exec_dg_st_for twice_gs (restrict_global_resolved_q cinit_ivl_st)"
     sigma_abs "fst twice_ctx_sol" "(cfg_exit twice_cfg, bot)" ivl_ctx_sg
 proof unfold_locales
   show "finite (intra twice_cfg)" by (rule twice_finE)
@@ -168,8 +174,8 @@ next
   show "part_post_solution
           (side_cfg_T_eff_keyed_seed_dg intra_predecessor_list (\<lambda>_. Global) route_abs_gen
              (routed_cmb Sabs Global) (routed_extra twice_cfg Sabs Seed Global) twice_cfg Sabs
-             (fun_of_exec_dg_st (bot::ivl exec_dg_st)) (fun_of_exec_dg_st cinit_ivl_st)
-             (fun_of_exec_dg_st (restrict_global_resolved_q cinit_ivl_st)))
+             (fun_of_exec_dg_st_for twice_gs (bot::ivl exec_dg_st)) (fun_of_exec_dg_st_for twice_gs cinit_ivl_st)
+             (fun_of_exec_dg_st_for twice_gs (restrict_global_resolved_q cinit_ivl_st)))
           (cfg_exit twice_cfg, bot) sigma_abs (fst twice_ctx_sol)"
     by (rule twice_ctx_pp_abs)
 next
@@ -203,13 +209,13 @@ lemma global_slot_shared:
   "ivl_ctx_sg (Inl (FunctionEntry ''twice'', ctx_call1)) ''Gx''
      = ivl_ctx_sg (Inl (FunctionEntry ''twice'', ctx_call2)) ''Gx''"
 proof -
-  have "lookup_exec_dg_st (locals (snd twice_ctx_sol (Inl (FunctionEntry ''twice'', ctx_call1)))) ''Gx''
-      = lookup_exec_dg_st (locals (snd twice_ctx_sol (Inl (FunctionEntry ''twice'', ctx_call2)))) ''Gx''"
+  have "twice_lookup_exec_dg_st (locals (snd twice_ctx_sol (Inl (FunctionEntry ''twice'', ctx_call1)))) ''Gx''
+      = twice_lookup_exec_dg_st (locals (snd twice_ctx_sol (Inl (FunctionEntry ''twice'', ctx_call2)))) ''Gx''"
     unfolding twice_ctx_sol_def twice_ctx_eqs_def by eval
   thus ?thesis
     unfolding ivl_ctx_sg_def
     by (simp add: callee_covered_call1 callee_covered_call2
-      fun_of_resolved_st_q_for_def)
+      fun_of_exec_dg_st_for_def fun_of_resolved_st_q_for_def)
 qed
 
 subsection \<open>SEED_G: the routed callee entry (enter edges)\<close>
@@ -227,19 +233,19 @@ text \<open>\<^bold>\<open>enter_route_exact.\<close>  The context a call routes
   so the routed context is exactly \<open>ctx_call1\<close> / \<open>ctx_call2\<close> --- the executable route agrees
   with the activation route \<^const>\<open>ivl_enterc\<close>.\<close>
 lemma enter_route_exact_call1:
-  assumes "s' = call_enter is_global (CallEdge dst [''p''] [VIMP_Syntax.N 3]) s"
+  assumes "s' = call_enter twice_gs (CallEdge dst [''p''] [VIMP_Syntax.N 3]) s"
   shows "ivl_enterc u ctx s' = ctx_call1"
 proof -
-  from assms have "s' = (enter_state is_global s)(''p'' := 3)"
+  from assms have "s' = (enter_state twice_gs s)(''p'' := 3)"
     by (simp add: call_enter_CallEdge bind_formals_def)
   thus ?thesis by (simp add: ivl_enterc_def ivl_decode_def ctx_call1_val)
 qed
 
 lemma enter_route_exact_call2:
-  assumes "s' = call_enter is_global (CallEdge dst [''p''] [VIMP_Syntax.N 10]) s"
+  assumes "s' = call_enter twice_gs (CallEdge dst [''p''] [VIMP_Syntax.N 10]) s"
   shows "ivl_enterc u ctx s' = ctx_call2"
 proof -
-  from assms have "s' = (enter_state is_global s)(''p'' := 10)"
+  from assms have "s' = (enter_state twice_gs s)(''p'' := 10)"
     by (simp add: call_enter_CallEdge bind_formals_def)
   thus ?thesis by (simp add: ivl_enterc_def ivl_decode_def ctx_call2_val)
 qed
@@ -264,19 +270,19 @@ text \<open>\<^bold>\<open>enter_route_exact for combine.\<close>  The callee co
   linked entered store is exactly the enter edge's \<^const>\<open>edge_step\<close> result, so this reuses
   \<open>enter_route_exact\<close>.\<close>
 lemma comb_route_call1:
-  assumes "call_enter_store is_global twice_cfg (Statement 2) s es"
+  assumes "call_enter_store twice_gs twice_cfg (Statement 2) s es"
   shows "ivl_enterc u c1 es = ctx_call1"
 proof -
-  have "es = call_enter is_global (CallEdge (Some ''x'') [''p''] [VIMP_Syntax.N 3]) s"
+  have "es = call_enter twice_gs (CallEdge (Some ''x'') [''p''] [VIMP_Syntax.N 3]) s"
     using assms twice_calls_shape unfolding call_enter_store_def by fastforce
   thus ?thesis by (rule enter_route_exact_call1)
 qed
 
 lemma comb_route_call2:
-  assumes "call_enter_store is_global twice_cfg (Statement 3) s es"
+  assumes "call_enter_store twice_gs twice_cfg (Statement 3) s es"
   shows "ivl_enterc u c1 es = ctx_call2"
 proof -
-  have "es = call_enter is_global (CallEdge (Some ''y'') [''p''] [VIMP_Syntax.N 10]) s"
+  have "es = call_enter twice_gs (CallEdge (Some ''y'') [''p''] [VIMP_Syntax.N 10]) s"
     using assms twice_calls_shape unfolding call_enter_store_def by fastforce
   thus ?thesis by (rule enter_route_exact_call2)
 qed
@@ -292,8 +298,9 @@ text \<open>The routed interval solution also interprets \<^locale>\<open>routed
   argument already used by \<open>comb_route_call1\<close> / \<open>comb_route_call2\<close>.  CALL and COMB then
   fall out as the locale's \<open>routed_context_call\<close> / \<open>routed_context_comb\<close>.\<close>
 
-interpretation twice_routed: routed_context Sabs is_global twice_cfg Global route_abs_gen
-    "fun_of_exec_dg_st (bot::ivl exec_dg_st)" "fun_of_exec_dg_st cinit_ivl_st" "fun_of_exec_dg_st (restrict_global_resolved_q cinit_ivl_st)"
+interpretation twice_routed: routed_context Sabs twice_gs twice_cfg Global route_abs_gen
+    "fun_of_exec_dg_st_for twice_gs (bot::ivl exec_dg_st)" "fun_of_exec_dg_st_for twice_gs cinit_ivl_st"
+    "fun_of_exec_dg_st_for twice_gs (restrict_global_resolved_q cinit_ivl_st)"
     sigma_abs "fst twice_ctx_sol" "(cfg_exit twice_cfg, bot)" ivl_ctx_sg Seed ivl_enterc
 proof (unfold_locales, goal_cases FinC SeedKey RouteAgree CallFwd CombFwd EnterAgree)
   case FinC
@@ -375,17 +382,17 @@ qed
 lemma ivl_ctx_sg_seed:
   assumes "(u, CallEdge dst xs es, FunctionEntry p, cont) \<in> calls twice_cfg"
     and "s \<in> \<lbrakk>ivl_ctx_sg (Inl (u, ctx))\<rbrakk>"
-  shows "call_enter is_global (CallEdge dst xs es) s
+  shows "call_enter twice_gs (CallEdge dst xs es) s
            \<in> \<lbrakk>ivl_ctx_sg (Inl (FunctionEntry p,
-                 ivl_enterc u ctx (call_enter is_global (CallEdge dst xs es) s)))\<rbrakk>"
+                 ivl_enterc u ctx (call_enter twice_gs (CallEdge dst xs es) s)))\<rbrakk>"
   by (rule twice_routed.routed_context_call[OF assms])
 
 lemma ivl_ctx_sg_comb:
   assumes "(cl, CallEdge dst pars args, FunctionEntry p, v) \<in> calls twice_cfg"
     and "s \<in> \<lbrakk>ivl_ctx_sg (Inl (cl, c1))\<rbrakk>"
     and "t \<in> \<lbrakk>ivl_ctx_sg (Inl (FunctionResult p, ivl_enterc cl c1 es))\<rbrakk>"
-    and "call_enter_store is_global twice_cfg cl s es"
-  shows "combine_collect is_global dst s t \<in> \<lbrakk>ivl_ctx_sg (Inl (v, c1))\<rbrakk>"
+    and "call_enter_store twice_gs twice_cfg cl s es"
+  shows "combine_collect twice_gs dst s t \<in> \<lbrakk>ivl_ctx_sg (Inl (v, c1))\<rbrakk>"
   by (rule twice_routed.routed_context_comb[OF assms])
 
 subsection \<open>Activation-indexed collecting soundness (obligation scaffold)\<close>
@@ -396,14 +403,14 @@ text \<open>Instantiating the generic \<open>activation_collect_sound\<close> at
   step / combine soundness, route consistency, and the \<open>ivl_ctx_sg_seed\<close> enter seed.\<close>
 
 theorem twice_activation_collect_sound:
-  "activation_collect is_global ivl_enterc bot twice_cfg (cinit_stores is_global) v ctx
+  "activation_collect twice_gs ivl_enterc bot twice_cfg (cinit_stores twice_gs) v ctx
      \<subseteq> \<lbrakk>ivl_ctx_sg (Inl (v, ctx))\<rbrakk>"
 proof (rule activation_collect_sound[where sg = ivl_ctx_sg and enterc = ivl_enterc
-        and seedc = bot and S = "cinit_stores is_global" and g = twice_cfg and gs = is_global])
+        and seedc = bot and S = "cinit_stores twice_gs" and g = twice_cfg and gs = twice_gs])
   \<comment> \<open>ENTRY_G --- mirrors \<open>twice_sound0\<close>: cinit stores lie in the seeded entry slot.\<close>
-  fix s assume "s \<in> cinit_stores is_global"
-  hence "s \<in> \<lbrakk>fun_of_exec_dg_st cinit_ivl_st\<rbrakk>" using cinit_le_cinit_ivl_st by blast
-  also have "\<lbrakk>fun_of_exec_dg_st cinit_ivl_st\<rbrakk> \<subseteq> \<lbrakk>locals (sigma_abs (Inl (cfg_entry twice_cfg, bot)))\<rbrakk>"
+  fix s assume "s \<in> cinit_stores twice_gs"
+  hence "s \<in> \<lbrakk>fun_of_exec_dg_st_for twice_gs cinit_ivl_st\<rbrakk>" using cinit_le_cinit_ivl_st by blast
+  also have "\<lbrakk>fun_of_exec_dg_st_for twice_gs cinit_ivl_st\<rbrakk> \<subseteq> \<lbrakk>locals (sigma_abs (Inl (cfg_entry twice_cfg, bot)))\<rbrakk>"
     by (rule gamma_state_mono[OF entry_locals_ge_s0d[OF entry_covered]])
   also have "\<dots> \<subseteq> \<lbrakk>ivl_ctx_sg (Inl (cfg_entry twice_cfg, bot))\<rbrakk>"
     unfolding ivl_ctx_sg_covered[OF entry_covered] by (rule gamma_state_sup_ub1)
@@ -420,9 +427,9 @@ next
   show "\<And>u dst pars args p cont c s.
         (u, CallEdge dst pars args, FunctionEntry p, cont) \<in> calls twice_cfg
         \<Longrightarrow> s \<in> \<lbrakk>ivl_ctx_sg (Inl (u, c))\<rbrakk>
-        \<Longrightarrow> call_enter is_global (CallEdge dst pars args) s
+        \<Longrightarrow> call_enter twice_gs (CallEdge dst pars args) s
              \<in> \<lbrakk>ivl_ctx_sg (Inl (FunctionEntry p,
-                    ivl_enterc u c (call_enter is_global (CallEdge dst pars args) s)))\<rbrakk>"
+                    ivl_enterc u c (call_enter twice_gs (CallEdge dst pars args) s)))\<rbrakk>"
     by (rule ivl_ctx_sg_seed)
 next
   \<comment> \<open>COMB --- return combine at the caller context \<open>c1\<close>: the resumed activation keeps its
@@ -431,8 +438,8 @@ next
         (cl, CallEdge dst pars args, FunctionEntry p, cont) \<in> calls twice_cfg
         \<Longrightarrow> s \<in> \<lbrakk>ivl_ctx_sg (Inl (cl, c1))\<rbrakk>
         \<Longrightarrow> t \<in> \<lbrakk>ivl_ctx_sg (Inl (FunctionResult p, ivl_enterc cl c1 es))\<rbrakk>
-        \<Longrightarrow> call_enter_store is_global twice_cfg cl s es
-        \<Longrightarrow> combine_collect is_global dst s t \<in> \<lbrakk>ivl_ctx_sg (Inl (cont, c1))\<rbrakk>"
+        \<Longrightarrow> call_enter_store twice_gs twice_cfg cl s es
+        \<Longrightarrow> combine_collect twice_gs dst s t \<in> \<lbrakk>ivl_ctx_sg (Inl (cont, c1))\<rbrakk>"
     by (rule ivl_ctx_sg_comb)
 qed
 
